CSL.v
@@ -1,0 +1,543 @@
+Require Import Logic.Eqdep.
+Require Import Bool.
+Require Import Arith.
+Require Import ZArith.
+Require Import String.
+Require Import QArith.
+Require Import Qcanon.
+
+Require Import Coq.Relations.Relations.
+
+Require ClassicalFacts.
+Require Export FunctionalExtensionality.
+Require Export ProofIrrelevance.
+
+Require Export Coq.ZArith.BinInt.
+Require Export String.
+
+Add LoadPath "../../src/cslsound".
+
+Require Export Vbase Varith Vlistbase Vlist Basic.
+
+Set Implicit Arguments.
+Unset Strict Implicit.
+
+Module PHeap.
+  Definition pheap := Z -> option (Qc * Z).
+
+  Definition is_pheap (h : pheap) : Prop :=
+    forall x, match h x with
+      | None => True
+      | Some (p, v) => 0 < p /\ p <= 1
+    end.
+  
+  Definition pdisj (h1 h2 : pheap) :=
+    forall (x : Z), match h1 x, h2 x with
+      | None, _ | _, None => True
+      | Some (p1, v1), some (p2, v2) =>
+        v1 = v2 /\ 0 < p1 + p2 /\ p1 + p2 <= 1
+    end.
+
+  Definition phplus (h1 h2 : pheap) : pheap :=
+    fun x => match h1 x with
+     | None => h2 x
+     | Some (p1, v1) => 
+       match h2 x with
+         | None => h1 x
+         | Some (p2, v2) => Some (p1 + p2, v1)
+       end
+     end.
+
+  Definition full_p : Qc := 1.
+  Definition emp_h : pheap := fun (n : Z) => None.
+
+  Definition fpdom (h : pheap) : Prop :=
+    forall (n : Z), match h n with
+      | None => True
+      | Some (p, v) => (p = full_p)%Qc
+    end.
+  
+  Lemma pdisjC : forall h1 h2, pdisj h1 h2 -> pdisj h2 h1.
+  Proof. 
+    unfold pdisj, pheap; intros h1 h2 hd x.
+    specialize (hd x).
+    destruct (h1 x), (h2 x); try tauto.
+    destruct p as [? ?], p0 as [? ?].
+    assert (q0 + q = q + q0) as heq by ring; rewrite heq.
+    destruct hd as [? [? ?]]; repeat split; auto.
+  Qed.
+
+  Lemma pdisj_empty1 : forall (h : pheap), pdisj emp_h h.
+    intros h; unfold emp_h, pdisj; simpl; eauto.
+  Qed.
+
+  Lemma pdisj_empty2 : forall (h : pheap), pdisj h emp_h.
+    now unfold emp_h, pdisj; simpl; intros h x; destruct (h x) as [[? ?] | ?].
+  Qed.
+
+  Definition upd (h : pheap) (x : Z) (v : Z) : pheap :=
+    fun (x' : Z) => if Zeq_bool x x' then Some (full_p, v) else h x'.
+
+  Definition empty_p := 0.
+
+  Lemma frac_contra1 : forall p : Qc, (p > empty_p)%Qc -> ~(full_p + p <= full_p)%Qc.
+  Proof.
+    unfold full_p; intros p hp hcontra.
+    apply (Qcle_minus_iff (1 + p) 1) in hcontra.
+    assert (1 + - (1 + p) = -p) as h by ring; rewrite h in hcontra; clear h.
+    apply Qcopp_le_compat in hcontra.
+    assert (- -p = p) as h by ring; rewrite h in hcontra; clear h.
+    assert (- 0 = 0) as h by ring; rewrite h in hcontra; clear h.
+    apply Qclt_not_le in hp; tauto.
+  Qed.
+
+  Lemma frac_contra2 : forall p, p > empty_p -> ~(p + full_p <= 1).
+  Proof.
+    intros ? ?; rewrite Qcplus_comm.
+    auto using frac_contra1.
+  Qed.
+  
+  Lemma pdisj_upd : forall (h h' : pheap) (H : is_pheap h) (H' : is_pheap h')
+    (x w v : Z), h x = Some (full_p, w) -> 
+    (pdisj (upd h x v) h' <-> pdisj h h').
+  Proof.
+    unfold pdisj, upd; ins.
+    split. 
+    - intros hp x0; specialize (hp x0); specialize (H x0); specialize (H' x0).
+      destruct (Zeq_bool x x0), (h x0) as [[? ?] | ], (h' x0) as [[? ?] | ]; eauto.
+      destruct hp as [? [? ?]],  H' as [? ?]; exfalso; eapply (@frac_contra1 q0); eauto.
+    - intros hp x0; specialize (hp x0); specialize (H x0); specialize (H' x0).
+      pose proof (Zeq_bool_if x x0); 
+      destruct (Zeq_bool x x0); subst;
+      destruct (h x0) as [[? ?] | ], (h' x0) as [[? ?] | ]; simpl; eauto;
+      inversion H0; subst.
+      destruct hp as [? [? ?]], H' as [? ?]; exfalso; eapply (@frac_contra1 q0); eauto.
+  Qed.
+
+  Lemma phplus_comm (h1 h2 : pheap) (H1 : is_pheap h1) (H2 : is_pheap h2) :
+    pdisj h1 h2 -> phplus h1 h2 = phplus h2 h1.
+  Proof.
+    intros hdisj; unfold is_pheap, pdisj, phplus in *; extensionality x.
+    repeat (match goal with [H : forall _ : Z, _ |- _] => specialize (H x) end).
+    destruct (h1 x) as [[? ?] | ], (h2 x) as [[? ?] | ]; eauto. 
+    destruct hdisj as [? [? ?]].
+    assert (q + q0 = q0 + q) by ring; congruence.
+  Qed.
+
+  Lemma plus_gt_0 : forall p1 p2 : Qc, 0 < p1 -> 0 < p2 -> 0 < p1 + p2.
+  Proof.
+    intros p1 p2 h1 h2.
+    assert (p2 < p1 + p2).
+    { apply Qclt_minus_iff.
+      cutrewrite (p1 + p2 + - p2 = p1); [eauto | ring]. }
+    apply (Qclt_trans _ p2 _); eauto.
+  Qed.
+
+  Lemma gt_0_plus : forall p p1 : Qc, 0 < p1 -> p < p + p1.
+  Proof.
+    intros p p1 h1.
+    apply Qclt_minus_iff.
+    cutrewrite (p + p1 + - p = p1); [eauto | ring].
+  Qed.
+
+  Lemma le1_weak : forall p p1 : Qc, 0 < p1 -> p + p1 <= 1 -> p <= 1.
+  Proof.
+    intros p p1 h1 hp.
+    apply Qclt_le_weak.
+    apply (Qclt_le_trans _ (p + p1) _); [apply gt_0_plus; eauto | eauto].
+  Qed.
+
+  Lemma pdisj_padd (h1 h2 h3 : pheap) (ph1 : is_pheap h1) (ph2 : is_pheap h2) (ph3 : is_pheap h3) :
+    pdisj h2 h3 -> pdisj h1 (phplus h2 h3) -> (pdisj h1 h2) /\ (pdisj h1 h3).
+  Proof.
+    unfold is_pheap, pdisj, phplus in *;
+    intros disj23 disj123; split; intros x; 
+    repeat (match goal with [H : forall _ : Z, _ |- _] => specialize (H x) end);
+    destruct (h1 x) as [[? ?] |], (h2 x) as [[? ?] |], (h3 x) as [[? ?] |];
+    destruct disj23 as [? [? ?]], disj123 as [? [? ?]], ph1 as [? ?], ph2 as [? ?], ph3 as [? ?];
+    repeat split; eauto using Qcplus_comm.
+
+    - apply plus_gt_0; eauto.
+    - cutrewrite (q + (q0 + q1) = (q + q0) + q1) in H4; [apply (@le1_weak _ q1); eauto | ring ].
+    - congruence.
+    - apply plus_gt_0; eauto.
+    - cutrewrite (q + (q0 + q1) = (q + q1) + q0) in H4; [apply (@le1_weak _ q0); eauto | ring ].
+  Qed.
+
+  Lemma pdisjE1 (h1 h2 h3 : pheap) (ph1 : is_pheap h1) (ph2 : is_pheap h2) (ph3 : is_pheap h3) :
+    pdisj h1 (phplus h2 h3) -> pdisj h2 h3 -> pdisj h1 h2.
+  Proof.
+    unfold is_pheap, pdisj, phplus in *;
+    intros h123 h23 x;
+    repeat (match goal with [H : forall _ : Z, _ |- _] => specialize (H x) end).
+    destruct (h1 x) as [[? ?] |], (h2 x) as [[? ?] |], (h3 x) as [[? ?] |],
+             ph1 as [? ?], ph2 as [? ?], ph3 as [? ?], h123 as [? [? ?]], h23 as [? [? ?]]; eauto.
+    repeat split; eauto using plus_gt_0.
+    cutrewrite (q + (q0 + q1) = (q + q0) + q1) in H7; [apply (@le1_weak _ q1); eauto | ring ].
+  Qed.
+
+  Lemma pdisjE2 (h1 h2 h3 : pheap) (ph1 : is_pheap h1) (ph2 : is_pheap h2) (ph3 : is_pheap h3) :
+    pdisj h1 (phplus h2 h3) -> pdisj h2 h3 -> pdisj h1 h3.
+  Proof.
+    unfold is_pheap, pdisj, phplus in *;
+    intros h123 h23 x;
+    repeat (match goal with [H : forall _ : Z, _ |- _] => specialize (H x) end).
+    destruct (h1 x) as [[? ?] |], (h2 x) as [[? ?] |], (h3 x) as [[? ?] |],
+             ph1 as [? ?], ph2 as [? ?], ph3 as [? ?], h123 as [? [? ?]], h23 as [? [? ?]]; eauto.
+    repeat split; eauto using plus_gt_0.
+    - congruence.
+    - cutrewrite (q + (q0 + q1) = (q + q1) + q0) in H7; [apply (@le1_weak _ q0); eauto | ring ].
+  Qed.
+
+  Lemma pdisj_padd_comm (h1 h2 h3 : pheap) (ph1 : is_pheap h1) (ph2 : is_pheap h2) (ph3 : is_pheap h3) :
+    pdisj h2 (phplus h1 h3) -> pdisj h1 h3 -> pdisj h1 (phplus h2 h3).
+  Proof.
+    unfold is_pheap, pdisj, phplus in *;
+    intros h123 h23 x;
+    repeat (match goal with [H : forall _ : Z, _ |- _] => specialize (H x) end).
+    destruct (h1 x) as [[? ?] |], (h2 x) as [[? ?] |], (h3 x) as [[? ?] |],
+             ph1 as [? ?], ph2 as [? ?], ph3 as [? ?], h123 as [? [? ?]], h23 as [? [? ?]]; eauto.
+    - cutrewrite (q + (q0 + q1) = q0 + (q + q1)); [ | ring].
+      repeat split; eauto.
+    - cutrewrite (q + q0 = q0 + q); [ | ring];
+      repeat split; eauto.
+  Qed.
+
+  Lemma pdisj_padd_expand 
+        (h1 h2 h3 : pheap) (ph1 : is_pheap h1) (ph2 : is_pheap h2) (ph3 : is_pheap h3) :
+    pdisj h1 h2 -> (pdisj (phplus h1 h2) h3 <-> (pdisj h1 (phplus h2 h3) /\ pdisj h2 h3)).
+  Proof.
+    unfold is_pheap, pdisj, phplus in *;
+    intros h12; split; [intros H; split; intros x | intros [H1 H2] x];
+    repeat (match goal with [H : forall _ : Z, _ |- _] => specialize (H x) end);
+    destruct (h1 x) as [[? ?] |], (h2 x) as [[? ?] |], (h3 x) as [[? ?] |],
+             ph1 as [? ?], ph2 as [? ?], ph3 as [? ?], h12 as [? [? ?]];
+    des; eauto;
+    repeat split; try congruence; eauto; 
+    try rewrite (Qcplus_assoc _ _ _); try rewrite (Qcplus_comm _ _); 
+    eauto using plus_gt_0.
+    - cutrewrite (q1 + (q + q0) = q + q0 + q1); [eauto | ring].
+    - cutrewrite (q + q0 + q1 = (q1 + q0) + q) in H10; [apply (@le1_weak _ q); eauto | ring].
+    - cutrewrite (q1 + (q + q0) = q + (q0 + q1)); [eauto | ring].
+  Qed.
+
+  Lemma padd_assoc
+        (h1 h2 h3 : pheap) (ph1 : is_pheap h1) (ph2 : is_pheap h2) (ph3 : is_pheap h3) :
+    pdisj h1 (phplus h2 h3) -> pdisj h2 h3 -> phplus (phplus h1 h2) h3 = phplus h1 (phplus h2 h3).
+  Proof.
+    unfold is_pheap, pdisj, phplus in *;
+    intros h123 h23; extensionality x;
+    repeat (match goal with [H : forall _ : Z, _ |- _] => specialize (H x) end);
+    destruct (h1 x) as [[? ?] |], (h2 x) as [[? ?] |], (h3 x) as [[? ?] |];
+    des; eauto.
+    cutrewrite (q + q0 + q1 = q + (q0 + q1)); [eauto | ring].
+  Qed.
+
+  Lemma padd_left_comm 
+        (h1 h2 h3 : pheap) (ph1 : is_pheap h1) (ph2 : is_pheap h2) (ph3 : is_pheap h3) :
+    pdisj h1 (phplus h2 h3) -> pdisj h2 h3 -> phplus h1 (phplus h2 h3) = phplus h2 (phplus h1 h3).
+  Proof.
+    unfold is_pheap, pdisj, phplus in *;
+    intros h123 h23; extensionality x;
+    repeat (match goal with [H : forall _ : Z, _ |- _] => specialize (H x) end);
+    destruct (h1 x) as [[? ?] |], (h2 x) as [[? ?] |], (h3 x) as [[? ?] |];
+    des; eauto.
+    - cutrewrite (q + (q0 + q1) = q0 + (q + q1)); [congruence | ring].
+    - cutrewrite (q + q0 = q0 + q); [congruence | ring].
+  Qed.
+  
+  Lemma padd_cancel
+        (h1 h2 h3 : pheap) (ph1 : is_pheap h1) (ph2 : is_pheap h2) (ph3 : is_pheap h3) :
+    phplus h1 h2 = phplus h1 h3 -> pdisj h1 h2 -> pdisj h1 h3 -> h2 = h3.
+    unfold is_pheap, pdisj, phplus in *;
+    intros heq h12 h13; extensionality x; pose proof  (equal_f heq x) as heq'; simpl in *; clear heq;
+    repeat (match goal with [H : forall _ : Z, _ |- _] => specialize (H x) end);
+    destruct (h1 x) as [[? ?] |], (h2 x) as [[? ?] |], (h3 x) as [[? ?] |];
+    des; eauto; try congruence.
+    - remember (q + q0) as q0'; remember (q + q1) as q1'.
+      inversion heq'. subst.
+      assert (q + q0 - q = q + q1 - q) by (rewrite H0; eauto).
+      cutrewrite (q + q0 - q = q0) in H; [| ring].
+      cutrewrite (q + q1 - q = q1) in H; [| ring].
+      congruence.
+    - remember (q + q0) as q'.
+      inversion heq'; subst.
+      assert (q + q0 - q = q - q) by (rewrite H0; eauto).
+      cutrewrite (q + q0 - q = q0) in H; [| ring].
+      cutrewrite (q - q = 0) in H; [| ring].
+      rewrite H in ph2.
+      inversion ph2.
+    - inversion heq'.
+      assert (q - q = (q + q0) - q) by (rewrite H0 at 1; eauto).
+      cutrewrite (q - q = 0) in H; [| ring].
+      cutrewrite (q + q0 - q = q0) in H; [| ring].
+      rewrite <- H in ph3; inversion ph3.
+  Qed.
+  
+  Definition ptoheap (ph : pheap) (h : heap) : Prop :=
+    forall (x : Z), match ph x with
+      | None => h x = None
+      | Some (p, v) => p = full_p /\ h x = Some v
+    end.
+
+  Lemma ptoD (ph1 ph2 : pheap) (h : heap) (hp1 : is_pheap ph1) (hp2 : is_pheap ph2) :
+    ptoheap ph1 h -> ptoheap ph2 h -> ph1 = ph2.
+  Proof.
+    unfold is_pheap, pdisj, phplus, ptoheap in *;
+    intros pto1 pto2; extensionality x;
+    repeat (match goal with [H : forall _ : Z, _ |- _] => specialize (H x) end);
+    destruct (ph1 x) as [[? ?] |], (ph2 x) as [[? ?] |];
+    des; eauto; try congruence.
+  Qed.
+
+Module Language.
+  Definition var := Z.
+  Definition stack := var -> Z.
+  Definition state := (stack * heap)%type.
+
+  Inductive exp := 
+  | Evar (x : var)
+  | Enum (n : Z)
+  | Eplus (e1: exp) (e2: exp).
+
+  Inductive bexp :=
+  | Beq (e1: exp) (e2: exp)
+  | Band (b1: bexp) (b2: bexp)
+  | Bnot (b: bexp).
+
+  Inductive cmd : Set :=
+  | Cskip
+  | Cassign (x: var) (e: exp)
+  | Cread (x: var) (e: exp)
+  | Cwrite (e1: exp) (e2: exp)
+  | Cseq (c1: cmd) (c2: cmd)
+  | Cif (b: bexp) (c1: cmd) (c2: cmd)
+  | Cwhile (b: bexp) (c: cmd)
+  | Cbarrier (j : nat).
+
+  Notation "'SKIP'" := Cskip.
+  Notation "x '::=' a" := (Cassign x a) (at level 60).
+  Notation "x '::=' '[' a ']'" := (Cread x a) (at level 60).
+  Notation "'[' a ']' '::=' e" := (Cwrite a e) (at level 60).
+  Notation "c1 ;; c2" := (Cseq c1 c2) (at level 80, right associativity).
+  Notation "'BARRIER' ( j )" := (Cbarrier j).
+
+  Fixpoint wait (c : cmd) : option (nat * cmd) :=
+    match c with
+      | SKIP | _ ::= _ | _ ::= [_] | [_] ::= _ | Cif _ _ _ | Cwhile _ _ => None
+      | BARRIER (j) => Some (j, Cskip)
+      | c1 ;; c2 =>
+        match wait c1 with
+          | Some (j, c1') => Some (j, c1' ;; c2)
+          | None => None
+        end
+    end.
+
+  Fixpoint edenot e s :=
+    match e with
+      | Evar v => s v
+      | Enum n => n
+      | Eplus e1 e2 => (edenot e1 s + edenot e2 s)%Z
+    end.
+  
+  Fixpoint bdenot b s : bool := 
+    match b with
+      | Beq e1 e2 => if Z.eq_dec (edenot e1 s) (edenot e2 s) then true else false
+      | Band b1 b2 => bdenot b1 s && bdenot b2 s
+      | Bnot b => negb (bdenot b s)
+    end.
+  
+  Reserved Notation "c '/' st  '==>s'  c' '/' st' " (at level 40, st at level 39, c' at level 39).
+  Inductive red: (cmd * state) -> (cmd * state) -> Prop := 
+  | red_Seq1: forall (c : cmd) (ss : state), (SKIP ;; c) / ss ==>s c / ss
+  | red_Seq2: forall (c1 : cmd) (ss : state) (c1' : cmd) (ss' : state) (c2 : cmd)
+                     (R: c1 / ss ==>s c1' / ss'), 
+                   (c1 ;; c2) / ss ==>s (c1' ;; c2) / ss'
+  | red_If1: forall (b : bexp) (c1 c2 : cmd) (ss : state) 
+                    (B: bdenot b (fst ss) = true), 
+                    (Cif b c1 c2) / ss ==>s c1 / ss
+  | red_If2: forall (b : bexp) (c1 c2 : cmd) (ss : state)
+                    (B: bdenot b (fst ss) = false),
+                    (Cif b c1 c2) / ss ==>s c2 / ss
+  | red_Loop: forall (b : bexp) (c : cmd) (ss : state), 
+                    (Cwhile b c) / ss ==>s (Cif b (Cseq c (Cwhile b c)) Cskip) / ss
+  | red_Assign: forall (x : var) (e : exp) ss ss' s h
+                       (EQ1: ss = (s, h))
+                       (EQ2: ss' = (upd s x (edenot e s), h)),
+                       (x ::= e) / ss ==>s Cskip / ss'
+  | red_Read: forall x e ss ss' s h v
+                     (EQ1: ss = (s, h))
+                     (RD: h (edenot e s) = Some v)
+                     (EQ2: ss' = (upd s x v, h)),
+                     (x ::= [e]) / ss ==>s Cskip / ss'
+  | red_Write: forall e1 e2 ss ss' s h
+                      (EQ1: ss = (s, h))
+                      (EQ2: ss' = (s, upd h (edenot e1 s) (Some (edenot e2 s)))),
+                      (Cwrite e1 e2) / ss ==>s Cskip / ss'
+   where  "c '/' st  '==>s'  c' '/' st' " := (red (c, st) (c', st')).
+
+  Definition multi_red : (cmd * state) -> (cmd * state) -> Prop := clos_refl_trans_1n _ red.
+  Notation "c '/' st  '==>s*'  c' '/' st' " := (multi_red (c, st) (c', st')) (at level 40, st at level 39, c' at level 39).
+  
+  Fixpoint accesses (c : cmd) (s : stack) := 
+    match c with
+      | Cskip => nil
+      | x ::= e => nil
+      | x ::= [e] => edenot e s :: nil
+      | [e] ::= e' => edenot e s :: nil
+      | c1 ;; c2 => accesses c1 s
+      | (Cif b c1 c2) => nil
+      | (Cwhile b c) => nil
+      | (Cbarrier _) => nil
+    end.
+
+  Fixpoint writes (c : cmd) (s : stack) :=
+    match c with
+      | Cskip => nil
+      | (x ::= e) => nil
+      | (x ::= [e]) => nil
+      | ([e] ::= e') => edenot e s :: nil
+      | (c1 ;; c2) => writes c1 s
+      | (Cif b c1 c2) => nil
+      | (Cwhile b c) => nil
+      | Cbarrier j => nil
+    end.
+  
+  Inductive aborts : cmd -> state -> Prop := 
+  | aborts_Seq : forall (c1 c2 : cmd) (ss : state) (A: aborts c1 ss), aborts (Cseq c1 c2) ss
+  | aborts_Read: forall x e ss
+                        (NIN: snd ss (edenot e (fst ss)) = None),
+                   aborts (Cread x e) ss
+  | aborts_Write: forall e1 e2 ss
+                         (NIN: snd ss (edenot e1 (fst ss)) = None),
+                    aborts (Cwrite e1 e2) ss.
+
+  Fixpoint barriers c :=
+    match c with
+      | Cskip => nil
+      | (Cassign x e) => nil
+      | (Cread x e) => nil
+      | (Cwrite e e') => nil
+      | (Cseq c1 c2) => barriers c1 ++ barriers c2
+      | (Cif b c1 c2) => barriers c1 ++ barriers c2
+      | (Cwhile b c) => barriers c
+      | Cbarrier j => j :: nil
+    end.
+
+  Definition wf_cmd c := disjoint_list (barriers c).
+
+  Module BigStep.
+    Reserved Notation " c '/' s '||' c' '/' s'" (at level 40, s at level 39, c' at level 39).
+    Inductive eval : cmd -> state -> option (nat * cmd) -> state -> Prop :=
+    | eval_Skip : forall (st : state), SKIP / st || None / st
+    | eval_Seq1 : forall (c1 c2 c1': cmd) (st st' : state) (j : nat),
+                    c1 / st || (Some (j, c1')) / st' ->
+                    (c1 ;; c2) / st || Some (j, c1' ;; c2) / st'
+    | eval_Seq2 : forall (c1 c2 : cmd) (c2' : option (nat * cmd)) (st st' st'' : state), 
+                    c1 / st || None / st' -> c2 / st' || c2' / st'' -> (c1 ;; c2) / st || c2' / st''
+    | eval_If1 : forall (b : bexp) (c1 c2 : cmd) (c1' : option (nat * cmd)) (st st' : state),
+                  bdenot b (fst st) = true -> c1 / st || c1' / st' ->
+                  (Cif b c1 c2) / st || c1' / st'
+    | eval_If2 : forall (b : bexp) (c1 c2 : cmd) (c2' : option (nat * cmd)) (st st' : state),
+                   bdenot b (fst st) = false -> c2 / st || c2' / st' ->
+                   (Cif b c1 c2) / st || c2' / st'
+    | eval_Loop : forall (b : bexp) (c : cmd) (c' : option (nat * cmd)) (st st' : state),
+                     (Cif b (c ;; (Cwhile b c)) Cskip) / st || c'/ st' ->
+                     (Cwhile b c) / st || c' / st'
+    | eval_Assign : forall (x : var) (e : exp) (st st' : state) s h,
+                      (st = (s, h)) -> (st' = (upd s x (edenot e s), h)) ->
+                      (x ::= e) / st || None / st'
+    | eval_Read : forall (x : var) (e : exp) (v : Z) (st st' : state) (s : stack) (h : heap),
+                    (st = (s, h)) -> (h (edenot e s) = Some v) ->
+                    (st' = (upd s x v, h)) ->
+                    (x ::= [e]) / st || None / st'
+    | eval_Write : forall e1 e2 ss ss' s h,
+                     (ss = (s, h)) ->
+                     (ss' = (s, upd h (edenot e1 s) (Some (edenot e2 s)))) ->
+                     (Cwrite e1 e2) / ss || None / ss'
+    | eval_Barrier : forall ss j,
+                       (Cbarrier j) / ss || Some (j, Cskip) / ss
+      where " c '/' s '||' c' '/' s'" := (eval c s c' s').
+    
+    Lemma red1_eval (x y : (cmd * state)) (st : state) : 
+      red x y -> (fst y) / (snd y) || None / st -> fst x / snd x || None / st.
+    Proof.
+      move=> H IH.
+      induction [st IH]H; ins; try do 10 (econstructor; eauto).
+      - inversion IH; subst.
+        econstructor; eauto.
+      - apply eval_If2; eauto.
+      - eapply eval_Assign; eauto.
+        inversion IH; subst; eauto.
+      - eapply eval_Read; eauto.
+        inversion IH; subst; eauto.
+      - eapply eval_Write; eauto.
+        inversion IH; subst; eauto.
+    Qed.
+
+    Corollary red1_eval' (c1 c2 : cmd) (st1 st2 st3 : state) : 
+      c1 / st1 ==>s c2 / st2 -> c2 / st2 || None / st3 -> c1 / st1 || None / st3.
+    Proof.
+      move=> H H'.
+      remember (c1, st1) as s1.
+      assert (c1 = fst s1) as h by (rewrite Heqs1; tauto); rewrite h in *; clear h.
+      assert (st1 = snd s1) as h by (rewrite Heqs1; tauto); rewrite h in *; clear h.
+      remember (c2, st2) as s2.
+      assert (c2 = fst s2) as h by (rewrite Heqs2; tauto); rewrite h in *; clear h.
+      assert (st2 = snd s2) as h by (rewrite Heqs2; tauto); rewrite h in *; clear h.
+      eapply red1_eval; eauto.
+    Qed.
+
+    Lemma eval__mred1 (c : cmd) (st st' : state) : 
+      c / st ==>s* Cskip / st' -> c / st || None / st'.
+      intros H. unfold multi_red in H.
+      remember (c, st) as s.
+      remember (SKIP, st') as s'.
+      assert (c = fst s) as h by (rewrite Heqs; tauto); rewrite h; clear h.
+      assert (st = snd s) as h by (rewrite Heqs; tauto); rewrite h; clear h.
+      assert (st' = snd s') as h by (rewrite Heqs'; tauto); rewrite h; clear h.
+      clear Heqs.
+       induction [Heqs'] H.
+      - move=>->; simpl; apply eval_Skip.
+      - move/IHclos_refl_trans_1n=>IH; clear IHclos_refl_trans_1n.
+        clear H0.
+        eapply red1_eval; eauto.
+    Qed.
+
+    Lemma eval_mred2 (c c' c'': cmd) (st st' : state) (j : nat) : 
+      c / st ==>s* c' / st' -> wait c' = Some (j, c'') ->
+      c / st || Some (j, c'') / st'.
+    Proof.
+      intros hs hwait.
+      unfold multi_red in hs.
+      remember (c, st) as s.
+      remember (c', st') as s'.
+      assert (c = fst s) as h by (rewrite Heqs; tauto); rewrite h; clear h.
+      assert (st = snd s) as h by (rewrite Heqs; tauto); rewrite h; clear h.
+      assert (st' = snd s') as h by (rewrite Heqs'; tauto); rewrite h; clear h.
+      clear Heqs.
+      induction [Heqs'] hs.
+      - intros ->.
+        induction [c'' j hwait]c'; move=> c'' j' hwait; inversion hwait.
+        + destruct (wait c'1); eauto.
+          * destruct p as (j'', c'); simpl in *.
+            apply eval_Seq1.
+            now apply IHc'1.
+          * inversion H0.
+        + apply eval_Barrier.
+      - move=>->; simpl in *.
+        assert ((c', st') = (c', st')) as IH by eauto; apply IHhs in IH; clear IHhs; simpl in *.
+        clear hs hwait c' c st.
+        induction [c'' IH]H; ins; try do 5 (econstructor; eauto).
+        + inversion IH; subst.
+          * apply eval_Seq1. 
+            apply IHred; eauto.
+          * eapply eval_Seq2; eauto.
+            eapply red1_eval'; eauto.
+        + apply eval_If2; eauto.
+        + inversion IH.
+        + inversion IH.
+        + inversion IH.
+    Qed.
+  End BigStep.
+End Language.
